added section RelativeTopTerminationCriterion

trunk/color/Term/WithArity/AMonAlg.v
@@ -86,12 +86,12 @@ Module MonotoneAlgebraResults (MA : MonotoneAlgebraType).
   Export MA.
   Require Import ACompat.
 
-  Notation IR_succ := (IR I succ).
-  Notation IR_succeq := (IR I succeq).
+  (*Notation IR_succ := (IR I succ).
+  Notation IR_succeq := (IR I succeq).*)
 
-  Notation term := (term Sig).
-  Notation rule := (rule Sig).
-  Notation rules := (list rule).
+  Notation term := (@term Sig).
+  Notation rule := (@rule Sig).
+  Notation rules := (@list rule).
 
   Lemma absorb_succ_succeq : absorb IR_succ IR_succeq.
 
@@ -119,11 +119,10 @@ Module MonotoneAlgebraResults (MA : MonotoneAlgebraType).
     exact monotone_succeq.
   Qed.
 
-
 (**********************************************************************)
 (** top termination (for DP setting) criterion with monotone algebras *)
 
-  Section TopTermination.
+  Section RelativeTopTermination.
 
     Variable R E : rules.
 
@@ -141,7 +140,138 @@ Module MonotoneAlgebraResults (MA : MonotoneAlgebraType).
       apply IR_WF. exact succ_wf.
     Qed.
 
-  End TopTermination.
+  End RelativeTopTermination.
+
+(**********************************************************)
+(** results and tactics for proving relative top termination 
+    of concrete examples. *)
+
+  Section RelativeTopTerminationCriterion.
+
+    Definition rule_partition R (R_dec : rel_dec R) (r : rule) := 
+      partition_by_rel R_dec (lhs r, rhs r).
+    Implicit Arguments rule_partition [R].
+
+    Lemma rule_partition_left : forall R (R_dec : rel_dec R) l r rs,
+      In (mkRule l r) (fst (partition (rule_partition R_dec) rs)) ->
+      partition_by_rel R_dec (l, r) = true.
+
+    Proof.
+      intros. unfold rule_partition in H.
+      set (w := partition_left
+        (fun r => partition_by_rel R_dec (lhs r, rhs r))). simpl in w.
+      change l with (lhs (mkRule l r)). change r with (rhs (mkRule l r)).
+      apply w with rs. assumption.
+    Qed.
+
+    Definition part_succeq := rule_partition succeq'_dec.
+    Definition part_succ := rule_partition succ'_dec.
+
+    Variable R E : rules.
+
+    Lemma rule_partition_complete : forall pf (R : rules),
+      let part := partition pf R in
+        red R << red (snd part) U red (fst part).
+
+    Proof.
+      clear R. intros. trans (red (snd part ++ fst part)). 
+      apply red_incl. unfold incl. intros.
+      destruct (partition_complete pf a R). assumption.
+      apply in_or_app. auto.
+      apply in_or_app. auto.
+      apply red_union.
+    Qed.
+
+    Lemma hd_rule_partition_complete : forall pf (R : rules),
+      let part := partition pf R in
+        hd_red R << hd_red (snd part) U hd_red (fst part).
+
+    Proof.
+      clear R. intros. trans (hd_red (snd part ++ fst part)).
+      apply hd_red_incl. unfold incl. intros.
+      destruct (partition_complete pf a R). assumption.
+      apply in_or_app. auto.
+      apply in_or_app. auto.
+      apply hd_red_union.
+    Qed.
+
+    Lemma partition_succ_compat : forall R,
+      compat IR_succ (fst (partition part_succ R)).
+
+    Proof.
+      clear R. intros R l r lr.
+      apply succ'_sub. apply partition_by_rel_true with MA.term succ'_dec.
+      apply rule_partition_left with R. assumption.
+    Qed.
+
+    Lemma partition_succeq_compat_fst : forall R,
+      compat IR_succeq (fst (partition part_succeq R)).
+
+    Proof.
+      clear R. intros R l r lr.
+      apply succeq'_sub. apply partition_by_rel_true with MA.term succeq'_dec.
+      apply rule_partition_left with R. assumption.
+    Qed.
+
+    Lemma partition_succeq_compat_snd : forall R,
+      snd (partition part_succeq R) = nil ->
+      compat IR_succeq (snd (partition part_succ R)).
+
+    Proof.
+      clear R. intros R Rpart l r lr.
+      apply succeq'_sub. apply partition_by_rel_true with MA.term succeq'_dec.
+      apply rule_partition_left with R. fold part_succeq.
+      deduce (partition_complete part_succeq (mkRule l r) R).
+      simpl in H. rewrite Rpart in H. destruct H.
+      apply partition_inright with part_succ. assumption.
+      assumption. destruct H.
+    Qed.
+
+    Lemma ma_relative_top_termination :
+      let E_ge := partition part_succeq E in
+      let R_gt := partition part_succ R in
+      let R_ge := partition part_succeq R in
+        snd R_ge = nil ->
+        snd E_ge = nil ->
+        WF (hd_red_mod E (snd R_gt)) ->
+        WF (hd_red_mod E R).
+
+    Proof.
+      intros. unfold hd_red_mod.
+      set (Rgt := fst R_gt) in *. set (Rge := snd R_gt) in *.
+      apply WF_incl with (red E # @ (hd_red Rge U hd_red Rgt)).
+      comp.
+      unfold Rge, Rgt, R_ge, R_gt. apply hd_rule_partition_complete.
+      apply wf_rel_mod_simpl. fold (red_mod E Rge). assumption.
+      apply WF_incl with (hd_red_mod (Rge ++ E) Rgt).
+      unfold hd_red_mod. comp.
+      apply incl_rtc.
+      trans (red Rge U red E). union. apply hd_red_incl_red.
+      apply red_union_inv.
+      apply ma_compat_hd_red_mod; trivial.
+      unfold Rgt, R_gt, part_succ. apply partition_succ_compat.
+      apply compat_app.
+      unfold Rge, R_gt. apply partition_succeq_compat_snd. assumption.
+      apply incl_compat with (fst E_ge ++ snd E_ge). unfold incl. intros.
+      apply in_or_app. unfold E_ge. apply partition_complete. exact H2.
+      rewrite H0. rewrite <- app_nil_end.
+      unfold E_ge. apply partition_succeq_compat_fst.
+    Qed.
+
+  End RelativeTopTerminationCriterion.
+
+(**********************************************************)
+(** tactics *)
+
+  Ltac do_prove_termination lemma := 
+    apply lemma; [solve [vm_compute; trivial] | idtac].
+
+  Ltac prove_termination :=  
+    match goal with
+    | |- WF (hd_red_mod ?E ?R) =>
+      do_prove_termination ma_relative_top_termination
+    | _ => fail "Unsupported termination problem type"
+   end.
 
 End MonotoneAlgebraResults.
 
@@ -287,6 +417,7 @@ Module ExtendedMonotoneAlgebraResults (EMA : ExtendedMonotoneAlgebraType).
 (**********************************************************)
 (** results and tactics for proving termination (as a special
     case of relative termination) of concrete examples. *)
+
   Section TerminationCriterion.
 
     Variable R : rules.
@@ -306,6 +437,9 @@ Module ExtendedMonotoneAlgebraResults (EMA : ExtendedMonotoneAlgebraType).
     Qed.
 
   End TerminationCriterion.
+
+(**********************************************************)
+(** tactics *)
 
   Ltac do_prove_termination lemma := 
     apply lemma; [solve [vm_compute; trivial] | idtac].
